thys/Pattern_Completeness/Pattern_Completeness_Multiset.thy
@@ -141,15 +141,15 @@ proof induct
 qed auto
 
 lemma mp_step_mset_vars: assumes "mp \<rightarrow>\<^sub>m mp'"
-  shows "tvars_mp (mp_mset mp) \<supseteq> tvars_mp (mp_mset mp')" 
+  shows "tvars_match (mp_mset mp) \<supseteq> tvars_match (mp_mset mp')" 
   using assms 
 proof induct 
   case *: (match_decompose' mp y f n mp' ys)
   {
     let ?mset = "mset :: _ \<Rightarrow> ('f,'v,'s)match_problem_mset"
     fix x
-    assume "x \<in> tvars_mp (mp_mset ((\<Sum>(t, l)\<in>#mp. ?mset (zip (args t) (map Var ys)))))" 
-    from this[unfolded tvars_mp_def, simplified]
+    assume "x \<in> tvars_match (mp_mset ((\<Sum>(t, l)\<in>#mp. ?mset (zip (args t) (map Var ys)))))" 
+    from this[unfolded tvars_match_def, simplified]
     obtain t l ti yi where tl: "(t,l) \<in># mp" and tiyi: "(ti,yi) \<in># ?mset (zip (args t) (map Var ys))" 
       and x: "x \<in> vars ti" 
       by auto
@@ -158,13 +158,13 @@ proof induct
     from tiyi[unfolded t] have "ti \<in> set ts"
       using set_zip_leftD by fastforce
     with x t have "x \<in> vars t" by auto
-    hence "x \<in> tvars_mp (mp_mset mp)" using tl unfolding tvars_mp_def by auto
+    hence "x \<in> tvars_match (mp_mset mp)" using tl unfolding tvars_match_def by auto
   }
-  thus ?case unfolding tvars_mp_def by force
-qed (auto simp: tvars_mp_def set_zip)
+  thus ?case unfolding tvars_match_def by force
+qed (auto simp: tvars_match_def set_zip)
 
 lemma mp_step_mset_steps_vars: assumes "(\<rightarrow>\<^sub>m)\<^sup>*\<^sup>* mp mp'"
-  shows "tvars_mp (mp_mset mp) \<supseteq> tvars_mp (mp_mset mp')" 
+  shows "tvars_match (mp_mset mp) \<supseteq> tvars_match (mp_mset mp')" 
   using assms by (induct, insert mp_step_mset_vars, auto)
 
 end
@@ -374,7 +374,7 @@ next
                 note get_var = wfvf[THEN conjunct1, rule_format]
                 note fun_case = wfvf[THEN conjunct2, rule_format]
                 (* fin-predicate: all variables in mp are of finite sort *)
-                define fin where "fin mp = Ball (tvars_mp (mp_mset mp)) (\<lambda> x. \<not> inf_sort (snd x))" for mp :: "('f,'v,'s) match_problem_mset"
+                define fin where "fin mp = Ball (tvars_match (mp_mset mp)) (\<lambda> x. \<not> inf_sort (snd x))" for mp :: "('f,'v,'s) match_problem_mset"
                 define p_fin where "p_fin = filter_mset fin p" 
                 define p_inf where "p_inf = filter_mset (Not o fin) p" 
                 have p_split: "p = p_inf + p_fin" unfolding p_fin_def p_inf_def by auto
@@ -395,13 +395,13 @@ next
                         case (Fun f ts)
                         with ty have "(Fun f ts, Var y) \<in> mp" by auto
                         from fun_case[OF _ this] mp obtain x where "(Var x, Var y) \<in> mp" "inf_sort (snd x)" by auto
-                        with fin[unfolded fin_def tvars_mp_def] mp tl have False by auto
+                        with fin[unfolded fin_def tvars_match_def] mp tl have False by auto
                         thus ?thesis by auto
                       qed auto
                       with ly show "(t,l) \<in> range (map_prod Var Var)" by auto
                     } note var_var = this
                     fix x assume xl: "(Var x, l) \<in> mp"
-                    then have xmp: "x \<in> tvars_mp mp" by (force simp: tvars_mp_def)
+                    then have xmp: "x \<in> tvars_match mp" by (force simp: tvars_match_def)
                     with wf[unfolded wf_pat_def wf_match_def, rule_format, OF mp]
                     have sxS: "snd x \<in> S" by auto
                     from mp xmp fin fin_def have "\<not>inf_sort (snd x)" by auto
@@ -429,7 +429,7 @@ next
                   from pat_inf_var_conflict[OF _ False this, folded p_split] no_step
                   obtain mp where mp: "mp \<in># p" and inf: "\<not> fin mp" and no_confl: "\<not> inf_var_conflict (mp_mset mp)" 
                     unfolding p_inf_def using impr by fastforce
-                  from inf[unfolded fin_def tvars_mp_def]
+                  from inf[unfolded fin_def tvars_match_def]
                   obtain t l x where tl: "(t,l) \<in># mp" and x: "x \<in> vars t" and inf: "inf_sort (snd x)" by auto
                   from get_var[OF _ tl] mp tl obtain y where ty: "(t, Var y) \<in># mp" by auto
                   have "\<exists> x. (Var x, Var y) \<in># mp \<and> inf_sort (snd x)" 
@@ -639,7 +639,7 @@ definition max_size :: "'s \<Rightarrow> nat" where
   "max_size s = (if s \<in> S \<and> \<not> inf_sort s then Maximum (size ` {t. t : s in \<T>(C)}) else 0)" 
 
 definition meas_finvars :: "('f,'v,'s)pat_problem_mset \<Rightarrow> nat" where
-  "meas_finvars = sum_ms (\<lambda> mp. sum (max_size o snd) (tvars_mp (mp_mset mp)))" 
+  "meas_finvars = sum_ms (\<lambda> mp. sum (max_size o snd) (tvars_match (mp_mset mp)))" 
 
 definition meas_symbols :: "('f,'v,'s)pat_problem_mset \<Rightarrow> nat" where
   "meas_symbols = sum_ms (sum_ms (\<lambda> (t,l). num_funs t))" 
@@ -669,26 +669,26 @@ lemma wf_rel_pats: "wf \<prec>mul"
   by (intro wf_inv_image wf_mult wf_rel_pat)
 
 
-lemma tvars_mp_fin: 
-  "finite (tvars_mp (mp_mset mp))"  
-  unfolding tvars_mp_def by auto
+lemma tvars_match_fin: 
+  "finite (tvars_match (mp_mset mp))"  
+  unfolding tvars_match_def by auto
 
 lemmas meas_def = meas_finvars_def meas_diff_def meas_symbols_def meas_setsize_def
 
-lemma tvars_mp_mono: "mp \<subseteq># mp' \<Longrightarrow> tvars_mp (mp_mset mp) \<subseteq> tvars_mp (mp_mset mp')" 
-  unfolding tvars_mp_def 
+lemma tvars_match_mono: "mp \<subseteq># mp' \<Longrightarrow> tvars_match (mp_mset mp) \<subseteq> tvars_match (mp_mset mp')" 
+  unfolding tvars_match_def 
   by (intro image_mono subset_refl set_mset_mono UN_mono)
 
-lemma meas_finvars_mono: assumes "tvars_mp (mp_mset mp) \<subseteq> tvars_mp (mp_mset mp')" 
+lemma meas_finvars_mono: assumes "tvars_match (mp_mset mp) \<subseteq> tvars_match (mp_mset mp')" 
   shows "meas_finvars {#mp#} \<le> meas_finvars {#mp'#}" 
-  using tvars_mp_fin[of mp'] assms
+  using tvars_match_fin[of mp'] assms
   unfolding meas_def by (auto intro: sum_mono2)
 
 lemma rel_mp_sub: "{# add_mset p mp#} \<succ> {# mp #}"
 proof - 
   let ?mp' = "add_mset p mp" 
   have "mp \<subseteq># ?mp'" by auto
-  from meas_finvars_mono[OF tvars_mp_mono[OF this]]
+  from meas_finvars_mono[OF tvars_match_mono[OF this]]
   show ?thesis unfolding meas_def rel_pat_def by auto
 qed
 
@@ -701,8 +701,8 @@ proof cases
   case *: (match_decompose f ts g ls mp'')
   have "meas_finvars {#mp'#} \<le> meas_finvars {#mp#}" 
   proof (rule meas_finvars_mono)
-    show "tvars_mp (mp_mset mp') \<subseteq> tvars_mp (mp_mset mp)" 
-      unfolding tvars_mp_def * using *(3) by (auto simp: set_zip set_conv_nth)
+    show "tvars_match (mp_mset mp') \<subseteq> tvars_match (mp_mset mp)" 
+      unfolding tvars_match_def * using *(3) by (auto simp: set_zip set_conv_nth)
   qed
   moreover 
   have id: "(case case x of (x, y) \<Rightarrow> (y, x) of (t, l) \<Rightarrow> f t l) = (case x of (a,b) \<Rightarrow> f b a)" for 
@@ -730,8 +730,8 @@ next
   moreover
   have "meas_finvars {#mp'#} \<le> meas_finvars {#mp#}" 
   proof (rule meas_finvars_mono)
-    show "tvars_mp (mp_mset mp') \<subseteq> tvars_mp (mp_mset mp)" 
-      unfolding tvars_mp_def * using *(3,6) 
+    show "tvars_match (mp_mset mp') \<subseteq> tvars_match (mp_mset mp)" 
+      unfolding tvars_match_def * using *(3,6) 
       by (auto simp: set_zip set_conv_nth) 
         (metis case_prod_conv nth_mem option.simps(3) root.elims term.sel(4) term.set_intros(4))
   qed
@@ -967,27 +967,27 @@ next
       have vars_\<tau>_var: "vars (\<tau> y) = (if x = y then set vs else {y})" for y unfolding \<tau> subst_def by auto
       have vars_\<tau>: "vars (t \<cdot> \<tau>) = vars t - {x} \<union> (if x \<in> vars t then set vs else {})" for t
         unfolding vars_term_subst image_comp o_def vars_\<tau>_var by auto
-      have tvars_mp_subst: "tvars_mp (mp_mset (?tau mp)) = 
-          tvars_mp (mp_mset mp) - {x} \<union> (if x \<in> tvars_mp (mp_mset mp) then set vs else {})" for mp
-        unfolding subst_defs subst_left_def tvars_mp_def
+      have tvars_match_subst: "tvars_match (mp_mset (?tau mp)) = 
+          tvars_match (mp_mset mp) - {x} \<union> (if x \<in> tvars_match (mp_mset mp) then set vs else {})" for mp
+        unfolding subst_defs subst_left_def tvars_match_def
         by (auto simp:vars_\<tau> split: if_splits prod.split)
-      have id1: "meas_finvars (?tau_mset {#mp#}) = (\<Sum>x\<in> tvars_mp (mp_mset (?tau mp)). max_size (snd x))"  for mp
+      have id1: "meas_finvars (?tau_mset {#mp#}) = (\<Sum>x\<in> tvars_match (mp_mset (?tau mp)). max_size (snd x))"  for mp
         unfolding meas_def subst_defs by auto
-      have id2: "meas_finvars {#mp#} = (\<Sum>x\<in>tvars_mp (mp_mset mp). max_size (snd x))"
+      have id2: "meas_finvars {#mp#} = (\<Sum>x\<in>tvars_match (mp_mset mp). max_size (snd x))"
         for mp :: "('f,'v,'s) match_problem_mset"
         unfolding meas_def subst_defs by simp
-      have eq: "x \<notin> tvars_mp (mp_mset mp) \<Longrightarrow> meas_finvars (?tau_mset {# mp #}) = meas_finvars {#mp#}" for mp
-        unfolding id1 id2 by (rule sum.cong[OF _ refl], auto simp: tvars_mp_subst)
+      have eq: "x \<notin> tvars_match (mp_mset mp) \<Longrightarrow> meas_finvars (?tau_mset {# mp #}) = meas_finvars {#mp#}" for mp
+        unfolding id1 id2 by (rule sum.cong[OF _ refl], auto simp: tvars_match_subst)
       {
         fix mp :: "('f,'v,'s) match_problem_mset"
         (* if x occurs in the matching problem, then we get a strict decrease *)
-        assume xmp: "x \<in> tvars_mp (mp_mset mp)" 
+        assume xmp: "x \<in> tvars_match (mp_mset mp)" 
         let ?mp = "(mp_mset mp)" 
-        have fin: "finite (tvars_mp ?mp)" by (rule tvars_mp_fin)
-        define Mp where "Mp = tvars_mp ?mp - {x}" 
-        from xmp have 1: "tvars_mp (mp_mset (?tau mp)) = set vs \<union> Mp" 
-          unfolding tvars_mp_subst Mp_def by auto
-        from xmp have 2: "tvars_mp ?mp = insert x Mp" and xMp: "x \<notin> Mp" unfolding Mp_def by auto
+        have fin: "finite (tvars_match ?mp)" by (rule tvars_match_fin)
+        define Mp where "Mp = tvars_match ?mp - {x}" 
+        from xmp have 1: "tvars_match (mp_mset (?tau mp)) = set vs \<union> Mp" 
+          unfolding tvars_match_subst Mp_def by auto
+        from xmp have 2: "tvars_match ?mp = insert x Mp" and xMp: "x \<notin> Mp" unfolding Mp_def by auto
         from fin have fin: "finite Mp" unfolding Mp_def by auto
         have "meas_finvars (?tau_mset {# mp #}) = sum (max_size \<circ> snd) (set vs \<union> Mp)" (is "_ = sum ?size _")
           unfolding id1 id2 using 1 by auto
@@ -1007,7 +1007,7 @@ next
         using eq[of mp] less[of mp] by linarith
 
       show "meas_finvars (?tau_mset {#mp#}) < meas_finvars {#mp#}" using x
-        by (intro less, unfold mp, force simp: tvars_mp_def)
+        by (intro less, unfold mp, force simp: tvars_match_def)
 
       show "meas_finvars (?tau_mset p) \<le> meas_finvars p" 
         unfolding subst_pat_problem_mset_def meas_finvars_def sum_ms_image o_def
@@ -1137,8 +1137,8 @@ next
     show ?case by simp
   next
     case *: (pat_instantiate n mp p x l s y t)
-    from *(2) have "x \<in> tvars_mp (mp_mset mp)" 
-      using conflicts(4)[of s t x] unfolding tvars_mp_def
+    from *(2) have "x \<in> tvars_match (mp_mset mp)" 
+      using conflicts(4)[of s t x] unfolding tvars_match_def
       by (auto intro!:term.set_intros(3))
     hence x: "x \<in> tvars_pat (pat_mset (add_mset mp p))" unfolding tvars_pat_def 
       using *(2) by auto
